tyding up

ulib/experimental/Steel.HigherReference.fst
@@ -103,50 +103,7 @@ let pts_to_ref_injective
                               (Some (Ghost.reveal v1, p1))
                               m
 
-let pts_to_framon (#a:Type) (r:ref a) (p:perm) : Lemma (is_frame_monotonic #a (fun v -> pts_to r p v)) =
-  let aux (x y : a) (m:mem) (f:slprop)
-    : Lemma (requires (interp (pts_to r p x `star` f) m /\ interp (pts_to r p y) m))
-            (ensures  (slimp (pts_to r p x) (pts_to r p y)))
-    =
-    let (ml, mr) = id_elim_star (pts_to r p x) f m in
-    assert (interp (pts_to r p x) ml);
-    assert (interp (pts_to r p x) m);
-    assert (interp (pts_to_raw r p y) m);
-    assert (interp (Mem.pts_to r (Some (Ghost.reveal x, p))) m);
-    assert (interp (Mem.pts_to r (Some (Ghost.reveal y, p))) m);
-    Mem.pts_to_join r (Some (Ghost.reveal x, p)) (Some (Ghost.reveal y, p)) m;
-    ()
-  in
-  Classical.forall_intro_4 (fun x y m -> Classical.move_requires (aux x y m))
-
-let pts_to_witinv (#a:Type) (r:ref a) (p:perm) : Lemma (witness_invariant #a (fun v -> pts_to r p v)) =
-  let aux (x y : a) (m:mem)
-    : Lemma (requires (interp (pts_to r p x) m /\ interp (pts_to r p y) m))
-            (ensures  (x == y))
-    =
-    Mem.pts_to_join r (Some (Ghost.reveal x, p)) (Some (Ghost.reveal y, p)) m
-  in
-  Classical.forall_intro_3 (fun x y -> Classical.move_requires (aux x y))
-
-let pts_to_framon' (#a:Type) (r:ref a) (p:perm) : Lemma (is_frame_monotonic (pts_to r p)) =
- (* copied from above + erased, sorry *)
-  let aux (x y : erased a) (m:mem) (f:slprop)
-    : Lemma (requires (interp (pts_to r p x `star` f) m /\ interp (pts_to r p y) m))
-            (ensures  (slimp (pts_to r p x) (pts_to r p y)))
-    =
-    let (ml, mr) = id_elim_star (pts_to r p x) f m in
-    assert (interp (pts_to r p x) ml);
-    assert (interp (pts_to r p x) m);
-    assert (interp (pts_to_raw r p y) m);
-    assert (interp (Mem.pts_to r (Some (Ghost.reveal x, p))) m);
-    assert (interp (Mem.pts_to r (Some (Ghost.reveal y, p))) m);
-    Mem.pts_to_join r (Some (Ghost.reveal x, p)) (Some (Ghost.reveal y, p)) m;
-    ()
-  in
-  Classical.forall_intro_4 (fun x y m -> Classical.move_requires (aux x y m))
-
-let pts_to_witinv' (#a:Type) (r:ref a) (p:perm) : Lemma (witness_invariant  (pts_to r p)) =
- (* copied from above + erased, sorry *)
+let pts_to_witinv (#a:Type) (r:ref a) (p:perm) : Lemma (witness_invariant  (pts_to r p)) =
   let aux (x y : erased a) (m:mem)
     : Lemma (requires (interp (pts_to r p x) m /\ interp (pts_to r p y) m))
             (ensures  (x == y))
@@ -155,6 +112,8 @@ let pts_to_witinv' (#a:Type) (r:ref a) (p:perm) : Lemma (witness_invariant  (pts
   in
   Classical.forall_intro_3 (fun x y -> Classical.move_requires (aux x y))
 
+let pts_to_framon (#a:Type) (r:ref a) (p:perm) : Lemma (is_frame_monotonic (pts_to r p)) =
+  pts_to_witinv r p
 
 let drop (p:slprop)
   : SteelT unit p (fun _ -> emp)
